

## Theorem 1: Dual Failure Law

**Theorem 1** (Dual Failure Law). *Let  $D(t), A(t) \in \mathbb{R}^n$  be continuously differentiable functions. Define the misalignment vector*

$$E(t) = D(t) - A(t).$$

*Then for all  $t$  such that  $E(t) \neq 0$ ,*

$$\frac{d}{dt}\|E(t)\| = \frac{E(t)}{\|E(t)\|} \cdot (\dot{D}(t) - \dot{A}(t)).$$

**Proof. Step 1: Norm Representation**

The Euclidean norm satisfies

$$\|E(t)\| = \sqrt{E(t) \cdot E(t)}.$$

Define

$$\phi(t) = E(t) \cdot E(t).$$

Then

$$\|E(t)\| = \sqrt{\phi(t)}.$$

**Step 2: Chain Rule**

$$\frac{d}{dt}\|E(t)\| = \frac{1}{2\sqrt{\phi(t)}}\phi'(t).$$

**Step 3: Differentiate the Inner Product**

$$\phi'(t) = 2E(t) \cdot \dot{E}(t).$$

Thus,

$$\frac{d}{dt}\|E(t)\| = \frac{1}{2\|E(t)\|} \cdot 2E(t) \cdot \dot{E}(t) = \frac{E(t) \cdot \dot{E}(t)}{\|E(t)\|}.$$

**Step 4: Substitute Error Dynamics**

Since

$$E(t) = D(t) - A(t),$$

we have

$$\dot{E}(t) = \dot{D}(t) - \dot{A}(t).$$

Therefore,

$$\frac{d}{dt}\|E(t)\| = \frac{E(t)}{\|E(t)\|} \cdot (\dot{D}(t) - \dot{A}(t)).$$

□